Weidenbach_Book/CDCL_CW_NOT.thy
@@ -5,11 +5,9 @@ begin
 declare upt.simps(2)[simp del]
 sledgehammer_params[verbose]
 
-interpretation cdcl_CW: dpll_state trail "\<lambda>S. clauses S \<union> learned_clauses S"
-  "\<lambda> M (_, N, U, k, D). (M, N, U, k, D)" "\<lambda> C (M, N, U, k, D). (M, N, insert C U, k, D)"
-  "\<lambda> C (M, N, U, k, D). (M, N - {C}, U - {C}, k, D)"
+interpretation cdcl_CW: dpll_state trail "\<lambda>S. clauses S \<union> learned_clss S"
+  "\<lambda>M (_, N, U, k, D). (M, N, U, k, D)" "\<lambda>C (M, N, U, k, D). (M, {}, C, k, D)"
   by unfold_locales auto
-
 
 lemma cdcl_bj_measure:
   assumes "cdcl_bj S T"
@@ -101,7 +99,7 @@ lemma rtranclp_skip_state_decomp:
   assumes "skip\<^sup>*\<^sup>* S T"
   shows
     "\<exists>M. trail S = M @ trail T \<and> (\<forall>m\<in>set M. \<not>is_marked m)" and
-    "T = (trail T, clauses S, learned_clauses S, backtrack_level S, conflicting S)"
+    "T = (trail T, clauses S, learned_clss S, backtrack_level S, conflicting S)"
   using assms by (induction rule: rtranclp_induct) (cases S;auto)+
 
 lemma fst_get_all_marked_decomposition_prepend_not_marked:
@@ -337,7 +335,7 @@ proof (rule ccontr)
 
   have
     S: "clauses S = N"
-       "learned_clauses S = U'"
+       "learned_clss S = U'"
        "backtrack_level S = k"
        "conflicting S = C_Clause (D + {#-L#})"
     using rtranclp_skip_state_decomp(2)[OF skip] unfolding U by auto
